src/proofs/no_slashable_attestations/supporting_lemmas/proofs_intermediate_steps.dfy
@@ -202,7 +202,7 @@ module Proofs_Intermediate_Steps
     lemma lemma_inv51_ind_inv(
         dv: DVState
     )    
-    requires inv27(dv)
+    requires inv_att_slashing_db_hist_keeps_track_of_only_rcvd_att_duties(dv)
     ensures inv51(dv)    
     {  
         forall hn: BLSPubkey, s: Slot 
@@ -216,7 +216,7 @@ module Proofs_Intermediate_Steps
                && s in dv.honest_nodes_states[hn].attestation_consensus_engine_state.att_slashing_db_hist.Keys
             {
                 var hn_state := dv.honest_nodes_states[hn];
-                assert inv27_body(hn_state);
+                assert inv_att_slashing_db_hist_keeps_track_of_only_rcvd_att_duties_body(hn_state);
                 assert inv51_body(hn_state, s);
             }
             else
